\documentclass[11pt,a4paper, 
swedish, english %% Make sure to put the main language last!
]{article}
\pdfoutput=1

%% Andréas's custom package 
%% (Will work for most purposes, but is mainly focused on physics.)
\usepackage{../custom_as}
\usepackage{mathrsfs}
\usepackage{eufrak}
\usepackage{cancel}
%% Figures can now be put in a folder: 
\graphicspath{ {figures/} %{some_folder_name/}
}
\usepackage{multicol}

%% If you want to change the margins for just the captions
\usepackage[size=small]{caption}

%% To add todo-notes in the pdf
\usepackage[%disable  %%this will hide all notes
]{todonotes} 

%% Change the margin in the documents
\usepackage[
%            top    = 3cm,              %% top margin
%            bottom = 3cm,              %% bottom margin
%            left   = 3cm, right  = 3cm %% left and right margins
]{geometry}

\newcommand{\enull}{\ensuremath{\varepsilon_{0}}}
\newcommand{\lD}{\ensuremath{\lambda_{\text{D}}}}
\newcommand{\wc}{\ensuremath{\omega_{\text{c}}}}
\newcommand{\rhom}{\ensuremath{{\rho_{\text{m}}}}}
\newcommand{\vA}{\ensuremath{v_{\text{A}}}}
\newcommand{\cs}{\ensuremath{c_{\text{s}}}}


%% If you want to chage the formatting of the section headers
\renewcommand{\thesubsection}{\arabic{section}.\Alph{subsection}}



%%%%%%%%%%%%%%%%%%%%%%%%%%%%%%%%%%%%%%%%%%%%%%%%%%%%%%%%%%%%%%%%%%%%%%
\begin{document}%% v v v v v v v v v v v v v v v v v v v v v v v v v v
%%%%%%%%%%%%%%%%%%%%%%%%%%%%%%%%%%%%%%%%%%%%%%%%%%%%%%%%%%%%%%%%%%%%%%


%%%%%%%%%%%%%%%%%%%% vvv Internal title page vvv %%%%%%%%%%%%%%%%%%%%%
\title{Assignment 4 \\
{\Large Plasma Physics -- RRY085}}
\author{Andréas Sundström}
\date\today%{2017-10-01}

\maketitle

%%%%%%%%%%%%%%%%%%%% ^^^ Internal title page ^^^ %%%%%%%%%%%%%%%%%%%%%
%% If you want a list of all todos
%\todolist

\section{Collisional diffusion in weakly ionized gas}
Assume that the electron-neutral interaction rate is
\begin{equation}
\nu_{\text{en}}=v_\ee N \sigma_\text{en},
\end{equation}
and the electron-ion interaction rate is
\begin{equation}
\nu_\text{ei}=\frac{\pi n e^4}{(4\pi\varepsilon_0 m_\ee)^2v_\ee^3},
\end{equation}
where $N$ is the neutral particle density and $n=n_\ee=n_\text{i}$ is
the electron/ion density. Then
\begin{equation}
\frac{\nu_\text{ei}}{\nu_{\text{en}}}
=\frac{n}{N}\frac{e^4}
{16\pi\varepsilon_0^2\sigma_\text{en}m_\ee^2 v_\ee^4}.
\end{equation}
If we take $\sigma_\text{en}=\unit[10^{-19}]{m^2}$ and an electron
energy of 1\,eV, then for the two different frequencies to be equal,
we would require 
\begin{equation}
\frac{n}{N}=
\frac{64\pi\varepsilon_0^2
\sigma_\text{en}\,\epsilon^2}{e^4}
\approx 0.06 = 6\,\%,
\end{equation}
where $\epsilon =m_\ee v_\ee^2/2$ is the energy of an electron.

Given air normal atmospheric pressure at room temperature with
$N=\unit[10^{26}]{m^{-3}}$ and weakly ionized plasma, and with the
same electron energy and $\sigma_\text{en}$. Then the diffusion
constant is roughly 
\begin{equation}
D=\frac{v_\ee^2}{\nu_\text{en}}
=\frac{v_\ee}{N\sigma_\text{en}}
=\frac{1}{N\sigma_\text{en}}\sqrt{\frac{2\epsilon}{m_\ee}}
\approx \unit[0.06]{m^2/s}.
\end{equation}
Since the plasma would be weakly ionized the electron-neutral
collision rate dominates. 



\section{Different heat conductivity models}
In this problem we're considering a 1D plasma system, and we will
investigate how different types of heat conductivity, $\chi$, will
affect the temperatures of the plasma. The temperature is given by the
ODE
\begin{equation}
\dv{r}\qty[\chi\dv{T}{r}]=-S(r)\qc
\eval{\dv{T}{r}}_{r=0}=0\qc
T(r=R)=T_0,
\end{equation}
where $S(r)=S_0(r-r_0)$ with $0<r_0<R$. With this information, we can
integrate both sides once
\begin{equation}\label{eq2:ODE}
\chi\dv{T}{r}=-S_0\Theta(r-r_0),
\end{equation}
where $\Theta$ is the Heaviside step function. There should also be a
constant of integration here, but with the initial condition
$\eval{\dv*{T}{r}}_{r=0}=0$, we see that said constant has to be~0
(unless $\chi$ diverges at $r\to0$).

Seeing that we will be dealing with the Heaviside step function, we
might as well state the following identity for finding primitive
functions to a product with the step function. Given some (smooth)
function $f(x')$ and the constants $x_1<x_0$, then 
\begin{equation}
\begin{aligned}
\int_{x_1}^{x}\dv{f}{x'}\Theta(x'-x_0)\id{x'}=&
\Theta(x-x_0)\int_{x_0}^{x}\dv{f}{x'}\id{x'}
=\Big(f(x)-f(x_0)\Big)\Theta(x-x_0).
\end{aligned}
\end{equation}
Obviously, any primitive function to $(\dv*{f}{x'})\Theta(x'-x_0)$
will be given by the RHS plus some arbitrary constant, thus
\begin{equation}\label{eq2:heaviside-int}
\int\dv{f}{x}\Theta(x-x_0)\id{x}
=C+\Big(f(x)-f(x_0)\Big)\Theta(x-x_0).
\end{equation}



\subsection{Classical transport}
If the heat conductivity follows classical heat transport, then
\begin{equation}
\chi(T)=\alpha_1T^{-1/2}
\end{equation}
and \eqref{eq2:ODE} is separable and we get
\begin{equation}
\int\alpha_1T^{-1/2}\id{T}=-\int S_0\Theta(r-r_0)\id{r},
\end{equation}
which, by \eqref{eq2:heaviside-int}, becomes
\begin{equation}
T^{1/2}(r)=\mathcal{T}^{1/2}
-\frac{S_0}{2\alpha_1}(r-r_0)\Theta(r-r_0).
\end{equation}
The constant of integration, $\mathcal{T}^{1/2}$, can easily be
determined by the boundary condition $T(r=R)=T_0$ which yields
\begin{equation}\label{eq2a:const}
T_0^{1/2}=\mathcal{T}^{1/2}-\frac{S_0}{2\alpha_1}(R-r_0)
\quad\Longleftrightarrow\quad
\mathcal{T}^{1/2}=T_0^{1/2}+\frac{S_0}{2\alpha_1}(R-r_0).
\end{equation}
This means that the temperature is
\begin{equation}
T(r)=\qty{T_0^{1/2}+\frac{S_0}{2\alpha_1}
\Big[(R-r_0)-(r-r_0)\Theta(r-r_0)\Big]}^2
\end{equation}
With words, the temperature stays constant $T=\mathcal{T}$, given by
\eqref{eq2a:const}, up until $r=r_0$ when the temperature drops 
``quadratically'' (along a parabola whose vertex is just to the right
of $r=R$) down to $T=T_0$ at $r=R$. 

\subsection{Neoclassical transport}
With neoclassical transportation, the heat conductivity is
\begin{equation}
\chi(r, T)=
\begin{cases}
\alpha_2 r_1^{-3/2}T^{-1/2}\qc&0\le r<r_1\\
\alpha_2 r^{-3/2}T^{-1/2}\qc& r_1\le r\le1,
\end{cases}
\end{equation}
where $0<r_1<r_0$. 

It is obvious that the temperature, just as before, will be constant
$T(r)=\mathscr{T}$ for $0\le r<r_0$ since $\dv*{T}{r}=0$ in that region. We
therefore only have to focus on the (overlapping) region
$r_1<r<R$. Here \eqref{eq2:ODE} 
%can be rewritten as 
%\begin{equation}
%\alpha_2T^{-1/2}\dv{T}{r}=-S_0\,r^{3/2}\Theta(r-r_0)=-S_0\,r^{3/2}
%\end{equation}
%which 
separates into
\begin{equation}
\alpha_2\int T^{-1/2}\id{T}=-S_0\int r^{3/2}\Theta(r-r_0) \id{r}.
\end{equation}
By \eqref{eq2:heaviside-int}, we therefore get
\begin{equation}
T^{1/2}(r)=\mathscr{T}^{1/2}
-\frac{S_0}{5\alpha_2}\qty(r^{5/2}-r_0^{5/2})\Theta(r-r_0).
\end{equation}
Once again, the constant $\mathscr{T}^{1/2}$ is determined by the boundary
condition $T(r=R)=T_0$, which yields
\begin{equation}
\mathscr{T}^{1/2}=T_0^{1/2}+
\frac{S_0}{5\alpha_2}\qty(R^{5/2}-r_0^{5/2}).
\end{equation}
Therefore
\begin{equation}
T(r)=\qty{T_0^{1/2}+\frac{S_0}{5\alpha_2}
\qty[\qty(R^{5/2}-r_0^{5/2})-\qty(r^{5/2}-r_0^{5/2})\Theta(r-r_0)]}^2.
\end{equation}
This is harder to describe with words, but the temperature is constant
$T=\mathscr{T}$ for $0\le r<r_0$ and then it starts dropping down to
$T(R)=T_0$. 

\subsection{Turbulent Gyro-Bohm like transport}
For turbulent Gyro-Bohm like transport, the heat conductivity is given
by
\begin{equation}
\chi(T)=\alpha_3 T^{3/2}.
\end{equation}
Thus, \eqref{eq2:ODE} separates into
\begin{equation}
\alpha_3\int T^{3/2}\id{T}=-S_0\int \Theta(r-r_0) \id{r}.
\end{equation}
As usual, \eqref{eq2:heaviside-int} gives
\begin{equation}
T^{5/2}(r)=\mathfrak{T}^{5/2}
-\frac{5S_0}{2\alpha_3}\qty(r-r_0)\Theta(r-r_0).
\end{equation}
The boundary condition $T(r=R)=T_0$ yields
\begin{equation}
\mathfrak{T}^{5/2}=T_0^{5/2}+
\frac{5S_0}{2\alpha_3}\qty(R-r_0)
\end{equation}
wherefore
\begin{equation}
T(r)=\qty{T_0^{5/2}+\frac{5S_0}{2\alpha_3}
\Big[(R-r_0)-(r-r_0)\Theta(r-r_0)\Big]}^{2/5}.
\end{equation}
Once again, this is constant $T=\mathfrak{T}$ for $0\le r<r_0$, and
then the temperature drops down to $T_0$ at $r=R$.

\subsection*{Limiting type of transport}
\begin{figure}
\centering
\includegraphics[width=12cm]{Q2.eps}
\caption{Temperature profiles for the three different types of heat
  transport, using the dimensionless values $S_0=10$, $R=1$,
  $r_0=0.1$, $T_0=0.1$, $\alpha_1=0.05$, $\alpha_2=0.5$ and
  $\alpha_3=5$. Also in the figure are numerical solutions to the
  differential equations shown as thick, dashed lines. Note the log
  scale on the vertical axis.}
\label{fig:transp}
\end{figure}

Using the dimensionless values $S_0=10$, $R=1$, $r_0=0.1$, $T_0=0.1$,
$\alpha_1=0.05$, $\alpha_2=0.5$ and $\alpha_3=5$. The core temperature
for the three different scenarios can be calculated to
\begin{equation}
\mathcal{T}\approx8\,160\qc
\mathscr{T}\approx18.5\qc
\mathfrak{T}\approx1.83,
\end{equation}
for classical, neoclassical and Gyro-Bohm transport
respectively. We clearly see that classical transport would have
yielded the, by almost three orders of magnitude, highest core
temperature, and that Gyro-Bohm yields the lowest core
temperature. This can also be seen in \figref{fig:transp}, where the
different temperature profiles have been plotted. 


\section{MHD stability}
Starting from the ideal MHD equations
\vspace{-22pt}
\begin{multicols}{2}
\begin{subequations}
\begin{align}
\label{eq:MHD-a}
&\rhom\dv{\vb*U}{t}=\vb*J\cross\vb*B-\grad P
\\ \label{eq:MHD-b}
&\pdv{\rhom}{t} +\div(\rhom\vb*U)=0
\\ \label{eq:MHD-c}
&\vb*E+\vb*U\cross\vb*B=0
\end{align}
\end{subequations}

\columnbreak

\addtocounter{equation}{-1}
\begin{subequations}
\addtocounter{equation}{3}
\begin{align}
\label{eq:MHD-d}
&\dv{t}\qty[\frac{P}{\rhom}]=0
\\ \label{eq:MHD-e}
&\curl\vb*B=\mu_0\vb*J %\qc \div\vb*B=0
\\ \label{eq:MHD-f}
&\curl\vb*E=-\pdv{\vb*B}{t}
\end{align}
\end{subequations}
\end{multicols}\noindent
and linearizing all variables around a flow-less, static equilibrium:
\begin{equation}
\vb*U=\vb0+\epsilon\vb*U_1 \qc
\vb*J=\vb*J_0+\epsilon\vb*J_1 \qc
\vb*B=\vb*B_0+\epsilon\vb*B_1 \qc
\ldots
\end{equation}
we want to find the MHD stability equation
\begin{equation}
\rhom_0\pdv[2]{\vb*U_1}{t}=\vb*F(\vb*U_1).
\end{equation}

It seems clear that we should start with \eqref{eq:MHD-a} and
linearize it. To order $\epsilon$ we get
\begin{equation}\label{eq:MHD-a-lin}
\rhom_0\dv{\vb*U_1}{t} = 
\vb*J_1\cross\vb*B_0+\vb*J_0\cross\vb*B_1-\grad P_1.
\end{equation}
Note that the term $\rhom_1\dv*{\vb*U_0}{t}=\vb0$, since
$\vb*U_0\equiv\vb0$. We further note that a full time derivative can
be written as
\begin{equation}
\dv{f}{t}=\pdv{f}{t}+\vb*U\vdot\grad{f},
\end{equation}
and when linearized
\begin{equation}\label{eq:dv-lin}
\dv{f_0}{t}+\epsilon\dv{f_1}{t}=
\pdv{f_0}{t}
+\epsilon\qty[\pdv{f_1}{t}+\vb*U_1\vdot\grad{f_0}]
+\order{\epsilon^2}.
\end{equation}
Once again $\vb*U_0\equiv\vb0$ was used.
In \eqref{eq:MHD-a-lin}, the full derivative therefore becomes
\begin{equation}\label{eq:dvU1}
\dv{\vb*U_1}{t}=\pdv{\vb*U_1}{t}+\vb*U_1\vdot\grad\vb*U_0
=\pdv{\vb*U_1}{t}.
\end{equation}
If we therefore operate with a \emph{partial} time derivative on
\eqref{eq:MHD-a-lin}, with \eqref{eq:dvU1} in mind, we get
\begin{equation}\label{eq:MHD-stab1}
\rhom_0\pdv[2]{\vb*U_1}{t} = 
\pdv{\vb*J_1}{t}\cross\vb*B_0
+\vb*J_0\cross\pdv{\vb*B_1}{t}-\grad \pdv{P_1}{t}.
\end{equation}
Here we have used the fact that the unperturbed state is static,
meaning that $X_0$ is constant in time for any variable $X$. We have
also used the fact that different (partial) derivatives commute, i.e. 
$\pdv*{(\grad P_1)}{t}=\grad\pdv*{P_1}{t}$.

From here we can use \eqref{eq:MHD-e}, \eqref{eq:MHD-f} and
\eqref{eq:MHD-c} to get 
\begin{equation}
\pdv{\vb*J_1}{t}=\frac{1}{\mu_0}\curl\pdv{\vb*B_1}{t}
=\frac{1}{\mu_0}\curl\qty[-\curl\vb*E_1]
=-\frac{1}{\mu_0}\curl\qty[\curl\qty(-\vb*U_1\cross\vb*B_0)].
\end{equation}
When linearizing \eqref{eq:MHD-c}, $\vb*U_0\equiv\vb0$ was used. 
Next up we can use \eqref{eq:MHD-f} and \eqref{eq:MHD-c} to get
\begin{equation}
\pdv{\vb*B_1}{t}=-\curl\vb*E_1
=-\curl\qty(-\vb*U_1\cross\vb*B_0).
\end{equation}
This, together with $\mu_0\vb*J_0=\curl\vb*B_0$, inserted into
\eqref{eq:MHD-stab1} yields
\begin{equation}\label{eq:MHD-stab2}
\begin{aligned}
\rhom_0\pdv[2]{\vb*U_1}{t} =& 
\frac{1}{\mu_0}\qty{\curl\qty[\curl\qty(\vb*U_1\cross\vb*B_0)]}
\cross\vb*B_0+\\
&+\frac{1}{\mu_0}(\curl\vb*B_0)\cross
\qty[\curl\qty(\vb*U_1\cross\vb*B_0)]
&-\grad \pdv{P_1}{t}.
\end{aligned}
\end{equation}

Now we turn our attention to the last term. We have a (partial) time
derivative of $P_1$, which suggests that we should use
\eqref{eq:MHD-d}. Note the full derivative meaning that we have to
use \eqref{eq:dv-lin},
%This results in
%\begin{equation}
%\dv{f_1}{t}=\pdv{f_1}{t}+\vb*U_1\vdot\grad{f_0},
%\end{equation}
where
\begin{equation}
f=\frac{P_0+\epsilon P_1}{(\rhom_0+\epsilon\rhom_1)^\gamma}
=\frac{P_0}{\rhom_0^\gamma}+\epsilon\qty[
\frac{P_1}{\rhom_0^\gamma} 
-\gamma\frac{P_0}{\rhom_0^\gamma}\frac{\rhom_1}{\rhom_0}].
\end{equation}
It is therefore clear that
\begin{equation}
f_0=\frac{P_0}{\rhom_0^\gamma}
\qc\qquad
f_1=\frac{P_1}{\rhom_0^\gamma} 
-\gamma\frac{P_0}{\rhom_0^{(\gamma+1)}}\rhom_1
\end{equation}
We can now see that the linearized \eqref{eq:MHD-d} becomes
\begin{equation}
\begin{aligned}
0=&\dv{f_1}{t}=\pdv{f_1}{t}+\vb*U_1\vdot\grad{f_0}\\
=&\frac{1}{\rhom_0^\gamma}\pdv{P_1}{t}
-\gamma\frac{P_0}{\rhom_0^{(\gamma+1)}}\pdv{\rhom_1}{t}
+\vb*U_1\vdot\qty[\frac{1}{\rhom_0^{\gamma}}\grad(P_0)
-\gamma\frac{P_0}{\rhom_0^{(\gamma+1)}}\grad(\rhom_0)],
\end{aligned}
\end{equation}
which can be rewritten as
\begin{equation}
\pdv{P_1}{t}=\gamma\frac{P_0}{\rhom_0}
\qty(\pdv{\rhom_1}{t}+\vb*U_1\vdot\grad\rhom_0)
-\vb*U_1\vdot\grad P_0.
\end{equation}
We now use \eqref{eq:MHD-b} and get
\begin{equation}
\pdv{\rhom_1}{t}=-\div(\rhom_0\vb*U_1)
=-\grad(\rhom_0)\vdot\vb*U_1
-\rhom_0\div\vb*U_1,
\end{equation}
which means that
\begin{equation}
\pdv{P_1}{t}=-\gamma P_0\div\vb*U_1
-\vb*U_1\vdot\grad P_0.
\end{equation}

We can now write \eqref{eq:MHD-stab2} as
\begin{equation}\label{eq:MHD-wave}
\begin{aligned}
\rhom_0\pdv[2]{\vb*U_1}{t} =& 
\frac{1}{\mu_0}\qty{\curl\qty[\curl\qty(\vb*U_1\cross\vb*B_0)]}
\cross\vb*B_0+\\
&+\frac{1}{\mu_0}(\curl\vb*B_0)\cross
\qty[\curl\qty(\vb*U_1\cross\vb*B_0)]
+\grad\qty[\gamma P_0\div\vb*U_1+\vb*U_1\vdot\grad P_0],
\end{aligned}
\end{equation}
which is the full MHD stability/wave equation. 


\section{Alfvén waves in infinite, homogeneous plasmas}
Now we want to find harmonic solutions,
$\vb*U_1\propto\vb*V_1(\vb*r)\ee^{\pm\ii\omega t}$, to
\eqref{eq:MHD-wave} in a uniform and static plasma. The static
assumption has already been heavily used in the previous problem to
derive \eqref{eq:MHD-wave}. The uniform assumption however, will help
us with the fact that $X_0$ is constant is space as well, for any
variable $X$; especially $\curl\vb*B_0=0$ and $\grad P_0=0$. With
these observations, \eqref{eq:MHD-wave} can be written as
\begin{equation}
-\rhom_0\omega^2\vb*V_1(\vb*r)
=\frac{1}{\mu_0}
\qty{\curl\qty[\curl\qty(\vb*V_1\cross\vb*B_0)]}\cross\vb*B_0
+\gamma P_0 \grad(\div\vb*V_1).
\end{equation}
This can be further simplified using the identity
\begin{equation}
\curl(\vb*F\cross\vb*G)
=(\vb*G\vdot\grad)\vb*F - (\vb*F\vdot\grad)\vb*G
+\vb*F(\div\vb*G) - \vb*G(\div\vb*F),
\end{equation}
which gives
$\curl(\vb*V_1\cross\vb*B_0)
=(\vb*B_0\vdot\grad)\vb*V_1 - \vb*B_0(\div\vb*V_1)$
since $\vb*B_0$ is constant.Thus
\begin{equation}
-\rhom_0\omega^2\vb*V_1(\vb*r)
=\frac{1}{\mu_0}
\qty{\curl\qty[(\vb*B_0\vdot\grad)\vb*V_1 
- \vb*B_0(\div\vb*V_1)]}\cross\vb*B_0
+\gamma P_0 \grad(\div\vb*V_1).
\end{equation}
Now we can also choose our coordinate system such that
$\vb*B_0=B_0\vu{z}$. This gives
\begin{equation}\label{eq4:MHD-wave_real}
-\omega^2\vb*V_1(\vb*r)
=\vA^2\qty{\curl\qty[\pdv{z}\vb*V_1 
- \vu{z}(\div\vb*V_1)]}\cross\vu{z}
+\cs^2 \grad(\div\vb*V_1),
\end{equation}
where
\begin{equation}
\vA^2:=\frac{B_0^2}{\mu_0\rhom_0}\qc\quad
\cs^2:=\frac{\gamma P_0}{\rhom_0}
\end{equation}
are the Alfvén velocity and the sound speed respectively.

Now, since the plasma is uniform and static, we can use the Fourier
transform
\begin{equation}
\vb*V_1(\vb*r)=\frac{1}{(2\pi)^3}
\int \rd^3k\, \vb*W(\vb*k)\,\ee^{+\ii\vb*k\vdot\vb*r},
\end{equation}
which means that $\grad\to\ii\vb*k$. We can furthermore rotate our
coordinate system such that $\vb*k=k_{||}\vu{z}+k_\perp\vu{y}$. We
can therefore write \eqref{eq4:MHD-wave_real} as
\begin{equation}
\begin{aligned}
-\omega^2\vb*W(\vb*k)
=&-\vA^2\qty{\vb*k\cross\qty[k_{||}\vb*W 
- (\vb*k\vdot\vb*W)\vu{z}]}\cross\vu{z}
-\cs^2 (\vb*k\vdot\vb*W)\vb*k\\
=&-\vA^2k_{||}[(\vb*k\cross\vb*W)\cross\vu{z}]
+\vA^2(\vb*k\vdot\vb*W)[(\vb*k\cross\vu{z})\cross\vu{z}]
-\cs^2 \vb*k(\vb*k\vdot\vb*W).
\end{aligned}
\end{equation}
Now we use the vector triple product identity
\begin{equation}
(\vb*a\cross\vb*b)\cross\vb*c=
(\vb*a\vdot\vb*c)\vb*b
-(\vb*b\vdot\vb*c)\vb*a,
\end{equation}
and move $\omega^2\vb*W$ to the RHS, which yields
\begin{equation}
\vb0=
\qty(\omega^2-\vA^2k_{||}^2)\vb*W+\vA^2k_{||}W_z\vb*k
-\qty[\qty(\vA^2+\cs^2)k_\perp\vu{y}+\cs^2k_{||}\vu{z}
](\vb*k\vdot\vb*W).
\end{equation}
This then simplifies down to
\begin{equation}\label{eq:MHD-unif-disp}
\begin{bmatrix}
\omega^2-\vA^2k_{||}^2 & 0 & 0 \\
0 & \omega^2-\vA^2k^2-\cs^2k_\perp^2 & -\cs^2k_{||}k_\perp\\
0 & -\cs^2k_{||}k_\perp & \omega^2 -\cs^2k_{||}^2
\end{bmatrix}
\begin{bmatrix}
W_x\\W_y\\W_z
\end{bmatrix}
=
\begin{bmatrix}
0\\0\\0
\end{bmatrix},
\end{equation}
where $k^2=|\vb*k|^2=k_{||}^2+k_\perp^2$. 

We get non-trivial solutions only when the determinant is 0, i.e.
\begin{equation}
\begin{aligned}
0=&\qty(\omega^2-\vA^2k_{||}^2)\qty[
\qty(\omega^2-\vA^2k^2-\cs^2k_\perp^2)\qty(\omega^2 -\cs^2k_{||}^2)
-\qty(-\cs^2k_{||}k_\perp)^2]\\
=&\qty(\omega^2-\vA^2k_{||}^2)\qty[\omega^4-
\qty(\vA^2k^2+\cs^2k_\perp^2+\cs^2k_{||}^2)\omega^2
+\vA^2k^2\cs^2k_{||}^2
+\cs^4k_\perp^2k_{||}^2-\qty(\cs^2k_{||}k_\perp)^2]\\
=&\qty(\omega^2-\vA^2k_{||}^2)\qty[
\omega^4-\qty(\vA^2+\cs^2)k^2\omega^2
+\vA^2\cs^2k^2k_{||}^2],
\end{aligned}
\end{equation}
which has the solutions
\begin{equation}\label{eq4:MHD-shear}
\omega^2=\vA^2k_{||}^2
\end{equation}
or
\begin{equation}
\begin{aligned}
\omega^2=&\frac{1}{2}\qty(\vA^2+\cs^2)k^2
\pm\sqrt{\frac{1}{4}\qty(\vA^2+\cs^2)^2k^4
-\vA^2\cs^2k^2k_{||}^2}\\
=&\frac{1}{2}\qty(\vA^2+\cs^2)k^2\qty[
1\pm\sqrt{1-\frac{4\vA^2\cs^2k_{||}^2}{\qty(\vA^2+\cs^2)^2k^2}}].
\end{aligned}
\end{equation}

We now see that \eqref{eq:MHD-unif-disp} has three different
modes. The first one being \eqref{eq4:MHD-shear}, which requires
$\vb*W=W\vu{x}$ and is therefore perpendicular to both $\vb*B_0$ and
$\vb*k$. Linearizing and Fourier transforming \eqref{eq:MHD-c} and
\eqref{eq:MHD-f} yields
\begin{equation}
\vb*B_1 = \frac{(\vb*W\cross\vb*B_0)\cross\vb*k}{\omega}
=\frac{\cancel{(\vb*k\vdot\vb*W)}\vb*B_0
-(\vb*k\vdot\vb*B_0)\vb*W}{\omega}
=-\frac{(\vb*k\vdot\vb*B_0)}{\omega}\vb*W.
\end{equation}
In other words, $\vb*B_1$ is perpendicular to $\vb*B_0$. This wave
mode shifts the the magnetic field lines perpendicularly to their
original direction (shearing), which is why it is called the
\emph{shear Alfvén wave}. We can further more see that if we
linearize and space (only) Fourier transform \eqref{eq:MHD-b}, we get 
\begin{equation}
0=\pdv{\rhom_1}{t} + \rhom_0\cancel{\vb*k\vdot\vb*W}
=\pdv{\rhom_1}{t}.
\end{equation}
That is since $\vb*k\vdot\vb*W=0$ (which implies $\div\vb*V_1=0$) the
density is constant to first order, i.e. the plasma does not compress
-- loosely takling it's \emph{incompressible} under this wave mode.



\section{Alfvén waves in a sheared magnetic field}




%%%%%%%%%%%%%%%%%%%%%%%%%%%%%%%%%%%%%%%%%%%%%%%%%%%%%%%%%%%%%%%%%%%%%%
\end{document}%% ^ ^ ^ ^ ^ ^ ^ ^ ^ ^ ^ ^ ^ ^ ^ ^ ^ ^ ^ ^ ^ ^ ^ ^ ^ ^ ^
%%%%%%%%%%%%%%%%%%%%%%%%%%%%%%%%%%%%%%%%%%%%%%%%%%%%%%%%%%%%%%%%%%%%%%
%  LocalWords: Alfvén MHD Bohm quadratically incompressible
